LeanSAT/LRAT/Actions.lean
@@ -3,7 +3,6 @@ Copyright Amazon.com, Inc. or its affiliates. All Rights Reserved.
 Released under Apache 2.0 license as described in the file LICENSE.
 Authors: Josh Clune
 -/
-import LeanSAT.Sat.Literal
 import LeanSAT.External.DimacsLRAT
 import LeanSAT.LRAT.Clause
 
